

This is a wonderful question! It's like a puzzle. In parts (a) and (b), we proved that the 1-form $\omega = \frac{1}{y} dx$ was "broken"â€”it wasn't a total differential (it wasn't "exact"), and its integral depended on the path.

This question now asks: **Can we "fix" it?** Can we add in the missing $dy$ and $dz$ pieces to create a _new_ 1-form that _is_ a total differential?

The answer is yes. The simplest and most elegant solution is:

-   $\omega_y = -\frac{x}{y^2}$
    
-   $\omega_z = 0$
    

Let's explore exactly how we get this and why it works.

---

### 1. How to Find the Components (The "Construction")

The goal is to find $\omega_y$ and $\omega_z$ such that the new form...

$$\omega = \frac{1}{y} dx + \omega_y dy + \omega_z dz$$

...is a total differential (an exact form).

By definition, an exact form is one that is the total differential $df$ of some scalar potential function $f(x, y, z)$.

$$df = \frac{\partial f}{\partial x} dx + \frac{\partial f}{\partial y} dy + \frac{\partial f}{\partial z} dz$$

Our strategy is to force this to be true. We can find the potential $f$ by using the one component we know, $\omega_x = \frac{1}{y}$.

Step 1: Identify the potential $f$ from $\omega_x$

We set the $dx$ components equal:

$$\frac{\partial f}{\partial x} = \omega_x = \frac{1}{y}$$

To find $f$, we integrate this expression with respect to $x$, treating $y$ and $z$ as constants:

$$f(x, y, z) = \int \frac{1}{y} dx = \frac{x}{y} + g(y, z)$$

This is the most general form of the potential $f$. The "$+C$" constant of integration isn't just a number, but can be any function $g(y, z)$ that only depends on $y$ and $z$, because $\frac{\partial g(y,z)}{\partial x} = 0$.

Step 2: Find $\omega_y$ and $\omega_z$ from this $f$

Now that we have our potential $f$, we can find the other components, $\omega_y$ and $\omega_z$, by simply taking the other partial derivatives of $f$:

$$\omega_y = \frac{\partial f}{\partial y} = \frac{\partial}{\partial y} \left( \frac{x}{y} + g(y, z) \right) = -\frac{x}{y^2} + \frac{\partial g}{\partial y}$$

$$\omega_z = \frac{\partial f}{\partial z} = \frac{\partial}{\partial z} \left( \frac{x}{y} + g(y, z) \right) = 0 + \frac{\partial g}{\partial z}$$

Step 3: Make the simplest choice

The question asks for suitable components, implying there are many valid answers. All of them depend on our choice of the arbitrary function $g(y, z)$.

The simplest and most common choice is to let $g(y, z)$ be a true constant, like $g(y, z) = 0$.

If we make this choice:

-   $\frac{\partial g}{\partial y} = 0$
    
-   $\frac{\partial g}{\partial z} = 0$
    

Plugging these in gives us our final answer:

$$\omega_y = -\frac{x}{y^2}$$

$$\omega_z = 0$$

So, our "fixed" 1-form, which is a total differential, is $\omega_{\text{fixed}} = \frac{1}{y} dx - \frac{x}{y^2} dy$.

---

### 2. Why This Works (The "Verification")

This works for two fundamental reasons, which are really two sides of the same coin.

#### Reason 1: It Works by Definition

We successfully found a potential function, $f(x, y, z) = \frac{x}{y}$. Let's find its total differential:

$$df = \frac{\partial}{\partial x}\left(\frac{x}{y}\right) dx + \frac{\partial}{\partial y}\left(\frac{x}{y}\right) dy + \frac{\partial}{\partial z}\left(\frac{x}{y}\right) dz$$

$$df = \left(\frac{1}{y}\right) dx + \left(-\frac{x}{y^2}\right) dy + (0) dz$$

This is exactly the new $\omega$ we just built. Since we have shown that $\omega = df$, it is, by definition, a total differential. The problem is solved.

#### Reason 2: We "Canceled the Curl"

In part (1.a), we showed that the original form $\omega_{\text{old}} = \frac{1}{y} dx$ was not closed. Its exterior derivative ("curl") was not zero:

$$d\omega_{\text{old}} = d\left(\frac{1}{y} dx\right) = d\left(\frac{1}{y}\right) \wedge dx = \left(-\frac{1}{y^2} dy\right) \wedge dx = \frac{1}{y^2} (dx \wedge dy)$$

This non-zero result $d\omega \neq 0$ was the reason it wasn't exact.

Now, look at the exterior derivative of the new piece we added, $\omega_{\text{new\_piece}} = -\frac{x}{y^2} dy$:

$$d(\omega_{\text{new\_piece}}) = d\left(-\frac{x}{y^2} dy\right) = -d\left(\frac{x}{y^2}\right) \wedge dy$$

$$= -\left( \frac{\partial(x/y^2)}{\partial x} dx + \frac{\partial(x/y^2)}{\partial y} dy \right) \wedge dy$$

$$= -\left( \frac{1}{y^2} dx - \frac{2x}{y^3} dy \right) \wedge dy$$

Distribute the wedge product:

$$= -\frac{1}{y^2} (dx \wedge dy) + \frac{2x}{y^3} (dy \wedge dy)$$

Since $dy \wedge dy = 0$, the second term vanishes:

$$d(\omega_{\text{new\_piece}}) = -\frac{1}{y^2} (dx \wedge dy)$$

This is the magic! The "badness" of the original form was $+\frac{1}{y^2} (dx \wedge dy)$. The new $dy$ component we added has an exterior derivative of exactly $-\frac{1}{y^2} (dx \wedge dy)$.

When we put them together, their "badness" cancels out:

$$d\omega_{\text{fixed}} = d(\omega_{\text{old}}) + d(\omega_{\text{new\_piece}})$$

$$d\omega_{\text{fixed}} = \left( \frac{1}{y^2} (dx \wedge dy) \right) + \left( -\frac{1}{y^2} (dx \wedge dy) \right) = 0$$

Because our new form $\omega_{\text{fixed}}$ is closed ($d\omega = 0$), it is guaranteed (in this simple space) to be exact (a total differential).

This is a deep insight: we "fixed" the 1-form by adding a new component whose "curl" was precisely engineered to cancel the "curl" of the original component.