

Hello! That's an excellent question. This is a classic and very important problem in statistical physics, and it's a perfect place to start. The problem asks us to explore a system where a property $X$ is described by an exponential decay.

Let's break it down step-by-step.

## Solving Your Statistical Physics Problem

The problem is given in three parts, so let's tackle them in order.

### 1. Finding the Normalization Constant ($\alpha$)

The Concept:

A probability density function (PDF), $p(X)$, describes the likelihood of finding a certain value $X$. If we add up all the probabilities for every possible value $X$ can take, the total probability must be 1 (or 100%). This is because the particle must have some value for its property $X$.

The "sum" for a continuous variable like $X$ is an integral over its entire domain. The problem states $X \in \mathbb{R}_0^+$, which means $X$ can be any value from $0$ to $\infty$.

This gives us the normalization condition:

$$\int_{0}^{\infty} p(X) dX = 1$$

The Calculation:

Now, we just substitute the function $p(X) = \alpha e^{-X}$ (from equation 4) into our normalization condition and solve for $\alpha$.

1.  Set up the integral:
    
    $$\int_{0}^{\infty} \alpha e^{-X} dX = 1$$
    
2.  Since $\alpha$ is just a constant, we can pull it out of the integral:
    
    $$\alpha \int_{0}^{\infty} e^{-X} dX = 1$$
    
3.  Now, we solve the integral $\int e^{-X} dX$. The antiderivative of $e^{-X}$ is $-e^{-X}$. We evaluate this from $0$ to $\infty$:
    
    $$\alpha \left[ -e^{-X} \right]_{0}^{\infty} = 1$$
    
4.  To evaluate at the limits, we take the value at infinity and subtract the value at zero:
    
    $$\alpha \left( \lim_{X \to \infty}(-e^{-X}) - (-e^{-0}) \right) = 1$$
    
5.  Let's look at these two terms:
    
    -   As $X$ becomes infinitely large, $e^{-X}$ (which is $\frac{1}{e^X}$) approaches $0$.
        
    -   $e^{-0}$ is just $e^0$, which is $1$.
        
6.  Plugging those values back in:
    
    $$\alpha \left( (0) - (-1) \right) = 1$$
    
    $$\alpha (1) = 1$$
    
    $$\alpha = 1$$
    

Result:

The normalization constant is $\alpha = 1$.

This means our fully normalized probability distribution is **$p(X) = e^{-X}$**. This is a very famous and important distribution in statistics, known as the **exponential distribution** (with a rate parameter of 1).

---

### 2. Calculating the Characteristic Function ($\Phi(k)$)

The Concept:

The characteristic function $\Phi(k)$ is a very powerful tool. You can think of it as a different way to represent the entire probability distribution. Its main superpower, which we'll see in part 3, is that it's a "moment-generating function." This means we can use it to easily find the average value $\langle X \rangle$, the average of the square $\langle X^2 \rangle$, and so on, just by taking derivatives.

The Calculation:

We are given the formula (Eq. 5) and we use our now-normalized PDF, $p(X) = e^{-X}$.

1.  Set up the integral:
    
    $$\Phi(k) = \int_{0}^{\infty} e^{-ikX} p(X) dX = \int_{0}^{\infty} e^{-ikX} e^{-X} dX$$
    
2.  We can combine the two exponential terms by adding their exponents:
    
    $$\Phi(k) = \int_{0}^{\infty} e^{-ikX - X} dX = \int_{0}^{\infty} e^{-(1 + ik)X} dX$$
    
3.  This integral is in the same form as $\int e^{-aX} dX$, where $a = (1 + ik)$. The solution is $\frac{e^{-aX}}{-a}$.
    
    $$\Phi(k) = \left[ \frac{e^{-(1 + ik)X}}{-(1 + ik)} \right]_{0}^{\infty}$$
    
4.  Now, we evaluate at the limits ($0$ and $\infty$):
    
    -   **At $X \to \infty$:** The term $e^{-(1 + ik)X}$ becomes $e^{-\infty} \cdot e^{-ik\infty}$. The $e^{-\infty}$ part goes to $0$ and "wins," making the entire numerator $0$.
        
    -   **At $X = 0$:** The term $e^{-(1 + ik) \cdot 0}$ becomes $e^0$, which is $1$.
        
5.  Putting it all together (value at $\infty$ - value at $0$):
    
    $$\Phi(k) = \left( 0 \right) - \left( \frac{e^{0}}{-(1 + ik)} \right)$$
    
    $$\Phi(k) = - \left( \frac{1}{-(1 + ik)} \right)$$
    
    $$\Phi(k) = \frac{1}{1 + ik}$$
    

Result:

The characteristic function is $\Phi(k) = \frac{1}{1 + ik}$. For the next step, it's very helpful to write this as $\Phi(k) = (1 + ik)^{-1}$.

---

### 3. Finding the Moments ($\langle X^m \rangle$)

The Concept:

"Moments" are the average values of the powers of $X$.

-   The 1st moment ($m=1$), $\langle X \rangle$, is the **mean** (the average value).
    
-   The 2nd moment ($m=2$), $\langle X^2 \rangle$, is the **mean-square**, which helps us find the variance (the "spread") of the distribution.
    

The problem gives us a "magic" formula to find any moment $\langle X^m \rangle$ without doing a new integral every time. We just take the $m$-th derivative of $\Phi(k)$!

$$\langle X^m \rangle = i^m \frac{d^m \Phi}{dk^m} \bigg|_{k=0}$$

(Here, $i$ is the imaginary unit, $i = \sqrt{-1}$, so $i^2 = -1$, $i^3 = -i$, etc.)

Let's find the first few moments to see the pattern.

Calculation for m = 1 (The Mean $\langle X \rangle$):

$$\langle X^1 \rangle = i^1 \frac{d^1 \Phi}{dk^1} \bigg|_{k=0} = i \frac{d}{dk} \left[ (1 + ik)^{-1} \right] \bigg|_{k=0}$$

1.  Find the derivative (using the chain rule):
    
    $$\frac{d}{dk} (1 + ik)^{-1} = -1 \cdot (1 + ik)^{-2} \cdot \frac{d}{dk}(1 + ik)$$
    
    $$= -1 \cdot (1 + ik)^{-2} \cdot (i) = -i(1 + ik)^{-2}$$
    
2.  Plug this back into the formula:
    
    $$\langle X \rangle = i \cdot \left[ -i(1 + ik)^{-2} \right] \bigg|_{k=0}$$
    
3.  Evaluate at k=0:
    
    $$\langle X \rangle = i \cdot \left[ -i(1 + 0)^{-2} \right] = i \cdot (-i \cdot 1) = -i^2$$
    
    Since $i^2 = -1$, we get:
    
    $$\langle X \rangle = -(-1) = 1$$
    
    So, the mean value of $X$ is 1.
    

Calculation for m = 2 (The Mean-Square $\langle X^2 \rangle$):

$$\langle X^2 \rangle = i^2 \frac{d^2 \Phi}{dk^2} \bigg|_{k=0} = (-1) \frac{d}{dk} \left[ \frac{d\Phi}{dk} \right] \bigg|_{k=0}$$

1.  Find the second derivative (we just differentiate our first derivative, $-i(1 + ik)^{-2}$):
    
    $$\frac{d^2 \Phi}{dk^2} = \frac{d}{dk} \left[ -i(1 + ik)^{-2} \right] = -i \cdot \frac{d}{dk} \left[ (1 + ik)^{-2} \right]$$
    
    $$= -i \cdot \left( -2 \cdot (1 + ik)^{-3} \cdot (i) \right)$$
    
    $$= (-i) \cdot (-2) \cdot (i) \cdot (1 + ik)^{-3} = (-i^2) \cdot (2) \cdot (1 + ik)^{-3}$$
    
    Since $-i^2 = 1$, this simplifies to:
    
    $$\frac{d^2 \Phi}{dk^2} = 2(1 + ik)^{-3}$$
    
2.  Plug this back into the formula:
    
    $$\langle X^2 \rangle = i^2 \cdot \left[ 2(1 + ik)^{-3} \right] \bigg|_{k=0}$$
    
3.  Evaluate at k=0:
    
    $$\langle X^2 \rangle = (-1) \cdot \left[ 2(1 + 0)^{-3} \right] = -1 \cdot (2 \cdot 1) = -2$$
    
    Wait! I made a sign error. Let's re-check the second derivative.
    
    $(-i) \cdot (-2) \cdot (i) = (-i \cdot i) \cdot (-2) = (-i^2) \cdot (-2) = (1) \cdot (-2) = -2$.
    
    Ah, there it is.
    
    $\frac{d^2 \Phi}{dk^2} = -2(1 + ik)^{-3}$
    
    Let's try step 3 again:
    
    $$\langle X^2 \rangle = i^2 \cdot \left[ -2(1 + ik)^{-3} \right] \bigg|_{k=0}$$
    
    $$\langle X^2 \rangle = (-1) \cdot \left[ -2(1 + 0)^{-3} \right] = (-1) \cdot (-2) = 2$$
    
    So, the mean-square value $\langle X^2 \rangle$ is 2.
    

Finding the Pattern:

Let's do one more, $\langle X^3 \rangle$:

-   The 3rd derivative is $\frac{d^3 \Phi}{dk^3} = \frac{d}{dk} [-2(1+ik)^{-3}] = -2 \cdot (-3) \cdot (1+ik)^{-4} \cdot (i) = 6i(1+ik)^{-4}$.
    
-   $\langle X^3 \rangle = i^3 \frac{d^3 \Phi}{dk^3} \bigg|_{k=0} = i^3 \cdot [6i(1+0)^{-4}] = i^3 \cdot 6i = 6i^4$.
    
-   Since $i^4 = (i^2)^2 = (-1)^2 = 1$, we get:
    
    $\langle X^3 \rangle = 6$.
    

Let's look at our results:

-   $\langle X^1 \rangle = 1 = 1!$
    
-   $\langle X^2 \rangle = 2 = 2!$
    
-   $\langle X^3 \rangle = 6 = 3!$
    

The pattern is clear! The $m$-th moment is $m$-factorial.

Result:

All non-vanishing moments are given by the general formula:

$$\langle X^m \rangle = m!$$

(where $m! = m \cdot (m-1) \cdot \dots \cdot 2 \cdot 1$)

---

## Summary of Our Results

Here is a quick summary of everything we found:

1.  **Normalization Constant:** $\alpha = 1$
    
2.  **Characteristic Function:** $\Phi(k) = \frac{1}{1 + ik}$
    
3.  **All Non-Vanishing Moments:** $\langle X^m \rangle = m!$
    

This was a fantastic exercise! We started with a physical observation (a property that decays exponentially) and, by using the rules of probability, we were able to find its normalization constant, its characteristic function, and a general formula for _all_ its average properties (moments).

Would you like to discuss what these moments tell us, for example, how to calculate the **variance** (the "spread") of the distribution using the first and second moments?